heap_lang/tests.v
@@ -4,14 +4,14 @@ From iris.heap_lang Require Import wp_tactics heap notation.
 Import uPred.
 
 Section LangTests.
-  Definition add : expr [] := (#21 + #21)%E.
-  Goal ∀ σ, prim_step add σ (#42) σ None.
+  Definition add : expr [] := (§21 + §21)%E.
+  Goal ∀ σ, prim_step add σ (§42) σ None.
   Proof. intros; do_step done. Qed.
-  Definition rec_app : expr [] := ((rec: "f" "x" := '"f" '"x") #0)%E.
+  Definition rec_app : expr [] := ((rec: "f" "x" := '"f" '"x") §0)%E.
   Goal ∀ σ, prim_step rec_app σ rec_app σ None.
   Proof. intros. rewrite /rec_app. do_step done. Qed.
-  Definition lam : expr [] := (λ: "x", '"x" + #21)%E.
-  Goal ∀ σ, prim_step (lam #21)%E σ add σ None.
+  Definition lam : expr [] := (λ: "x", '"x" + §21)%E.
+  Goal ∀ σ, prim_step (lam §21)%E σ add σ None.
   Proof. intros. rewrite /lam. do_step done. Qed.
 End LangTests.
 
@@ -22,9 +22,9 @@ Section LiftingTests.
   Implicit Types Φ : val → iPropG heap_lang Σ.
 
   Definition heap_e  : expr [] :=
-    let: "x" := ref #1 in '"x" <- !'"x" + #1 ;; !'"x".
+    let: "x" := ref §1 in '"x" <- !'"x" + §1 ;; !'"x".
   Lemma heap_e_spec E N :
-     nclose N ⊆ E → heap_ctx N ⊑ #> heap_e @ E {{ λ v, v = #2 }}.
+     nclose N ⊆ E → heap_ctx N ⊑ #> heap_e @ E {{ λ v, v = §2 }}.
   Proof.
     rewrite /heap_e=>HN. rewrite -(wp_mask_weaken N E) //.
     wp eapply wp_alloc; eauto. apply forall_intro=>l; apply wand_intro_l.
@@ -36,15 +36,15 @@ Section LiftingTests.
 
   Definition FindPred : val :=
     rec: "pred" "x" "y" :=
-      let: "yp" := '"y" + #1 in
+      let: "yp" := '"y" + §1 in
       if: '"yp" < '"x" then '"pred" '"x" '"yp" else '"y".
   Definition Pred : val :=
     λ: "x",
-      if: '"x" ≤ #0 then -^FindPred (-'"x" + #2) #0 else ^FindPred '"x" #0.
+      if: '"x" ≤ §0 then -^FindPred (-'"x" + §2) §0 else ^FindPred '"x" §0.
 
   Lemma FindPred_spec n1 n2 E Φ :
     n1 < n2 → 
-    Φ #(n2 - 1) ⊑ #> FindPred #n2 #n1 @ E {{ Φ }}.
+    Φ §(n2 - 1) ⊑ #> FindPred §n2 §n1 @ E {{ Φ }}.
   Proof.
     revert n1. wp_rec=>n1 Hn.
     wp_let. wp_op. wp_let. wp_op=> ?; wp_if.
@@ -53,7 +53,7 @@ Section LiftingTests.
     - assert (n1 = n2 - 1) as -> by omega; auto with I.
   Qed.
 
-  Lemma Pred_spec n E Φ : ▷ Φ #(n - 1) ⊑ #> Pred #n @ E {{ Φ }}.
+  Lemma Pred_spec n E Φ : ▷ Φ §(n - 1) ⊑ #> Pred §n @ E {{ Φ }}.
   Proof.
     wp_lam. wp_op=> ?; wp_if.
     - wp_op. wp_op.
@@ -63,7 +63,7 @@ Section LiftingTests.
   Qed.
 
   Lemma Pred_user E :
-    (True : iProp) ⊑ #> let: "x" := Pred #42 in ^Pred '"x" @ E {{ λ v, v = #40 }}.
+    (True : iProp) ⊑ #> let: "x" := Pred §42 in ^Pred '"x" @ E {{ λ v, v = §40 }}.
   Proof.
     intros. ewp apply Pred_spec. wp_let. ewp apply Pred_spec. auto with I.
   Qed.
@@ -73,7 +73,7 @@ Section ClosedProofs.
   Definition Σ : gFunctors := #[ heapGF ].
   Notation iProp := (iPropG heap_lang Σ).
 
-  Lemma heap_e_closed σ : {{ ownP σ : iProp }} heap_e {{ λ v, v = #2 }}.
+  Lemma heap_e_closed σ : {{ ownP σ : iProp }} heap_e {{ λ v, v = §2 }}.
   Proof.
     apply ht_alt. rewrite (heap_alloc nroot ⊤); last by rewrite nclose_nroot.
     apply wp_strip_pvs, exist_elim=> ?. rewrite and_elim_l.
